NumLean/Data/FinHTuple.lean
@@ -3,5 +3,5 @@ module
 public import NumLean.Data.FinHTuple.Basic
 public import NumLean.Data.FinHTuple.Fold
 public import NumLean.Data.FinHTuple.FinHTupleMap
+public import NumLean.Data.FinHTuple.Pretty
 @[expose] public section
-
