Tests/FloatTensor.lean
@@ -1,0 +1,33 @@
+module
+
+public import NumLean
+public import NumLean.Data.Scalars.Float64.RealModel
+-- public meta import NumLean.Data.FinHTuple.Pretty
+
+@[expose] public section
+
+open NumLean
+
+namespace FloatTensor
+
+
+/-- info: [2.000000,4.000000,6.000000,8.000000] -/
+#guard_msgs in
+#eval! ⊞[1.0,2,3,4] + ⊞[1.0,2,3,4]
+
+/-- info: 2.0 • ⊞[1.0, 2, 3, 4] : Float^[4] -/
+#guard_msgs in
+#check 2.0 • ⊞[1.0,2,3,4]
+
+/-- info: ⊞[1.0, 2, 3, 4] - ⊞[100.0, 0, 0, 0] : Float^[4] -/
+#guard_msgs in
+#check ⊞[1.0,2,3,4] - ⊞[100.0,0,0,0]
+
+/-- info: ⊞[[1.0, 2], [3, 4]] - ⊞[[100.0, 0], [0, 0]] : Float^[2, 2] -/
+#guard_msgs in
+#check ⊞[[1.0,2],[3,4]] - ⊞[[100.0,0],[0,0]]
+
+-- missing product of TensorIndexType
+/-- info: ⊞[[1.0, 2], [3, 4]] : Float^[2, 2] -/
+#guard_msgs in
+#check ⊞[[1.0,2],[3,4]]
